%
\newcommand{\dpos}{-4}
\newcommand{\mhpos}{\numexpr \dpos+1}
\newcommand{\mlpos}{\numexpr \dpos-1}
\begin{figure}
\begin{centering}
\begin{tikzpicture}[>=triangle 45]
  \node (PH) at (0,0) {\framebox{$\PH$}};
  \node (CH) at (0,\dpos) {\framebox{$\CH$}};
  \node (PV) at (4,0) {\framebox{$\PV$}};
  \node (CV) at (4,\dpos) {\framebox{$\CV$}};
  \node (CVp) at (2,\mhpos) {\framebox{$\CVp$}};
  \node (CHp) at (2,\mlpos) {\framebox{$\CHp$}};
  \draw[->,bend right=10] 
      (PH) to
      node[left,color=blue!70]{relax} 
      (CH);
  \draw[->,bend right=10] 
      (CH) to
      node[right,color=violet!70]{restrict} 
      (PH);
  \draw[->, bend right=10]
      (PV) to
      node[left,color=violet!70]{relax} 
      (CV);
  \draw[->,bend right=10]
      (CV) to
      node[right, color=blue!70]{restrict} 
      (PV);
  \draw[->,bend left=15]
      (CH) to
      node[above left,color=black!70]{lift}
      (CVp);
  \draw[->,bend left=15, color=red]
      (CVp) to
      node[above right]{$\F^*$}
      (CV);
  \draw[->,bend left=15]
      (CV) to
      node[below right,color=black!70]{lift}
      (CHp);
  \draw[->,bend left=15,color=red]
      (CHp) to
      node[below left]{$\F$}
      (CH);
\end{tikzpicture}
\caption{Diagram of the proof}
\label{fig:proof}
\end{centering}
\end{figure}

